@prefix chicsch:        <http://www.chic.eu/ontologies/resource#> .
@prefix rdf: <http://www.w3.org/1999/02/22-rdf-syntax-ns#> .
@prefix rdfs: <http://www.w3.org/2000/01/rdf-schema#> .
@prefix mo: <http://www.chic.eu/ontologies/some-model-ontology#>

# p.grenon @ ucl.ac.uk

### Provision for a highlevel schema defining:
# a class of models

<http://www.chic.eu/ontologies/resource#ModellingEntity>
  a rdfs:Class ;
  rdfs:label "Modelling entity" ;
  rdfs:comment "An instance of ModellingEntity is an entity such as a model or one of its parts." . 

# title or name 

<http://www.chic.eu/ontologies/resource#hasName>
  a rdf:Property ;
  rdfs:label "has name" ;
  rdfs:comment "link between an and a readable name" ;
  rdfs:domain <http://www.chic.eu/ontologies/resource#Object> ;
  rdfs:range rdfs:Literal .

# description 

<http://www.chic.eu/ontologies/resource#parameterhasUnits-string>
  a rdf:Property ;
  rdfs:label "has description" ;
  rdfs:comment "link between an and a readable description" ;
  rdfs:domain <http://www.chic.eu/ontologies/resource#Object> ;
  rdfs:range rdfs:Literal .

<http://www.chic.eu/ontologies/resource#interpreted-type>
  a rdf:Property ;
  rdfs:label "has input parameter" ;
  rdfs:comment "link between a model and an input parameter" ;
  rdfs:domain <http://www.chic.eu/ontologies/resource#Object> ;
  rdfs:range rdfs:Resource .
  
### Modelling 

<http://www.chic.eu/ontologies/resource#Object>
  a rdfs:Class ;
  rdfs:label "Object" ;
  rdfs:comment "An instance of Object is an entity." . 

<http://www.chic.eu/ontologies/resource#Model>
  a rdfs:Class ;
  rdfs:label "Model" ;
  rdfs:comment "An instance of Model is a model." ;
  rdfs:subClassOf <http://www.chic.eu/ontologies/resource#ModellingEntity> . 
  
# a class of parameters

<http://www.chic.eu/ontologies/resource#ModelParameter>
  a rdfs:Class ;
  rdfs:label "Model parameter" ;
  rdfs:comment "An instance of ModelParameter is a parameter in a model." ;
  rdfs:subClassOf <http://www.chic.eu/ontologies/resource#ModellingEntity> . 
  
# a relationship between models and parameters

<http://www.chic.eu/ontologies/resource#modelHasParameter>
  a rdf:Property ;
  rdfs:label "has parameter" ;
  rdfs:comment "link between a model and a parameter" ;
  rdfs:domain <http://www.chic.eu/ontologies/resource#Model> ;
  rdfs:range <http://www.chic.eu/ontologies/resource#ModelParameter> .

<http://www.chic.eu/ontologies/resource#modelHasParameter-Input>
  a rdf:Property ;
  rdfs:subPropertyOf <http://www.chic.eu/ontologies/resource#modelHasParameter> ; 
  rdfs:label "has input parameter" ;
  rdfs:comment "link between a model and an input parameter" ;
  rdfs:domain <http://www.chic.eu/ontologies/resource#Model> ;
  rdfs:range <http://www.chic.eu/ontologies/resource#ModelParameter> .

<http://www.chic.eu/ontologies/resource#modelHasParameter-Output>
  a rdf:Property ;
  rdfs:subPropertyOf <http://www.chic.eu/ontologies/resource#modelHasParameter> ; 
  rdfs:label "has input parameter" ;
  rdfs:comment "link between a model and an output parameter" ;
  rdfs:domain <http://www.chic.eu/ontologies/resource#Model> ;
  rdfs:range <http://www.chic.eu/ontologies/resource#ModelParameter> .

# ALT: a relationship between parameters and models

<http://www.chic.eu/ontologies/resource#parameterOfModel>
  a rdf:Property ;
  rdfs:label "has parameter" ;
  rdfs:comment "link between a parameter and a model of which it is a parameter" ;
  rdfs:domain <http://www.chic.eu/ontologies/resource#Model> ;
  rdfs:range <http://www.chic.eu/ontologies/resource#ModelParameter> .

<http://www.chic.eu/ontologies/resource#inputParameterOfModel>
  a rdf:Property ;
  rdfs:subPropertyOf <http://www.chic.eu/ontologies/resource#parameterOfModel> ; 
  rdfs:label "has input parameter" ;
  rdfs:comment "link between a parameter and a model where the parameter is an input parameter" ;
  rdfs:domain <http://www.chic.eu/ontologies/resource#ModelParameter> ;
  rdfs:range <http://www.chic.eu/ontologies/resource#Model> .

<http://www.chic.eu/ontologies/resource#outputParameterOfModel>
  a rdf:Property ;
  rdfs:subPropertyOf <http://www.chic.eu/ontologies/resource#parameterOfModel> ; 
  rdfs:label "has input parameter" ;
  rdfs:comment "link between a parameter and a model where the parameter is an output parameter" ;
  rdfs:domain <http://www.chic.eu/ontologies/resource#ModelParameter> ;
  rdfs:range <http://www.chic.eu/ontologies/resource#Model> .

  
# a relationship to explicit parameter attributes and a class of parameter attributes (input output)
# or specialised types of parameters 

<http://www.chic.eu/ontologies/resource#hasFileByFilename>
  a rdf:Property ;
  rdfs:label "" ;
  rdfs:comment "links a parameter to the filename in which the parameter is specified" ;
  rdfs:domain <http://www.chic.eu/ontologies/resource#ModelParameter> ;
  rdfs:range rdfs:Literal .

# units associated to parameters 

<http://www.chic.eu/ontologies/resource#parameterhasUnits-string>
  a rdf:Property ;
  rdfs:label "has units" ;
  rdfs:comment "link between a parameter and a unit (string name)" ;
  rdfs:domain <http://www.chic.eu/ontologies/resource#ModelParameter> ;
  rdfs:range rdfs:Literal .
  
<http://www.chic.eu/ontologies/resource#parameterhasUnits>
  a rdf:Property ;
  rdfs:label "has units" ;
  rdfs:comment "link between a parameter and a unit (a class in the Unit Ontology)" ;
  rdfs:domain <http://www.chic.eu/ontologies/resource#ModelParameter> ;
  rdfs:range rdfs:Resource .
  # specialisation of <http://purl.obolibrary.org/obo/UO_0000000> .
  # Unit 

<http://www.chic.eu/ontologies/resource#parameterhasDatatype>
  a rdf:Property ;
  rdfs:label "has units" ;
  rdfs:comment "link between a parameter and a datatype, for example xsd or other" ;
  rdfs:domain <http://www.chic.eu/ontologies/resource#ModelParameter> ;
  rdfs:range rdfs:Resource .


#### Supporting the categorisation of models along perspectives: 
## a slot associates a model to a concept in a perspective, this can be used to define a corresponding class of models

<http://www.chic.eu/ontologies/resource#objectCharacterisedBy>
  a rdf:Property ;
  rdfs:label "characterised by" ;
  rdfs:comment "Associates an Object to a concept" ;
  rdfs:domain <http://www.chic.eu/ontologies/resource#Object> ;
  rdfs:range rdfs:Resource .

<http://www.chic.eu/ontologies/resource#hasPositionIn-1>
  a rdf:Property ;
  rdfs:label "characterised by according to CHIC perspective 1" ;
  rdfs:comment "Associates a model to a concept according to CHIC perspective 1" ;
    rdfs:subPropertyOf <http://www.chic.eu/ontologies/resource#objectCharacterisedBy> ; 
  rdfs:domain <http://www.chic.eu/ontologies/resource#Model> ;
  rdfs:range rdfs:Resource .

<http://www.chic.eu/ontologies/resource#hasPositionIn-2>
  a rdf:Property ;
  rdfs:label "characterised by according to CHIC perspective 2" ;
  rdfs:comment "Associates a model to a concept according to CHIC perspective 2" ;
    rdfs:subPropertyOf <http://www.chic.eu/ontologies/resource#objectCharacterisedBy> ; 
  rdfs:domain <http://www.chic.eu/ontologies/resource#Model> ;
  rdfs:range rdfs:Resource .

<http://www.chic.eu/ontologies/resource#hasPositionIn-3>
  a rdf:Property ;
  rdfs:label "characterised by according to CHIC perspective 3" ;
  rdfs:comment "Associates a model to a concept according to CHIC perspective 3" ;
    rdfs:subPropertyOf <http://www.chic.eu/ontologies/resource#objectCharacterisedBy> ; 
  rdfs:domain <http://www.chic.eu/ontologies/resource#Model> ;
  rdfs:range rdfs:Resource .
  
<http://www.chic.eu/ontologies/resource#hasPositionIn-4>
  a rdf:Property ;
  rdfs:label "characterised by according to CHIC perspective 4" ;
  rdfs:comment "Associates a model to a concept according to CHIC perspective 4" ;
    rdfs:subPropertyOf <http://www.chic.eu/ontologies/resource#objectCharacterisedBy> ; 
  rdfs:domain <http://www.chic.eu/ontologies/resource#Model> ;
  rdfs:range rdfs:Resource .
  
<http://www.chic.eu/ontologies/resource#hasPositionIn-5>
  a rdf:Property ;
  rdfs:label "characterised by according to CHIC perspective 5" ;
  rdfs:comment "Associates a model to a concept according to CHIC perspective 5" ;
    rdfs:subPropertyOf <http://www.chic.eu/ontologies/resource#objectCharacterisedBy> ; 
  rdfs:domain <http://www.chic.eu/ontologies/resource#Model> ;
  rdfs:range rdfs:Resource .
  
<http://www.chic.eu/ontologies/resource#hasPositionIn-6>
  a rdf:Property ;
  rdfs:label "characterised by according to CHIC perspective 6" ;
  rdfs:comment "Associates a model to a concept according to CHIC perspective 6" ;
    rdfs:subPropertyOf <http://www.chic.eu/ontologies/resource#objectCharacterisedBy> ; 
  rdfs:domain <http://www.chic.eu/ontologies/resource#Model> ;
  rdfs:range rdfs:Resource .
  
<http://www.chic.eu/ontologies/resource#hasPositionIn-7>
  a rdf:Property ;
  rdfs:label "characterised by according to CHIC perspective 7" ;
  rdfs:comment "Associates a model to a concept according to CHIC perspective 7" ;
    rdfs:subPropertyOf <http://www.chic.eu/ontologies/resource#objectCharacterisedBy> ; 
  rdfs:domain <http://www.chic.eu/ontologies/resource#Model> ;
  rdfs:range rdfs:Resource .
  
<http://www.chic.eu/ontologies/resource#hasPositionIn-8>
  a rdf:Property ;
  rdfs:label "characterised by according to CHIC perspective 8" ;
  rdfs:comment "Associates a model to a concept according to CHIC perspective 8" ;
    rdfs:subPropertyOf <http://www.chic.eu/ontologies/resource#objectCharacterisedBy> ; 
  rdfs:domain <http://www.chic.eu/ontologies/resource#Model> ;
  rdfs:range rdfs:Resource .
  
<http://www.chic.eu/ontologies/resource#hasPositionIn-9>
  a rdf:Property ;
  rdfs:label "characterised by according to CHIC perspective 9" ;
  rdfs:comment "Associates a model to a concept according to CHIC perspective 9" ;
    rdfs:subPropertyOf <http://www.chic.eu/ontologies/resource#objectCharacterisedBy> ; 
  rdfs:domain <http://www.chic.eu/ontologies/resource#Model> ;
  rdfs:range rdfs:Resource .
  
<http://www.chic.eu/ontologies/resource#hasPositionIn-10>
  a rdf:Property ;
  rdfs:label "characterised by according to CHIC perspective 10" ;
  rdfs:comment "Associates a model to a concept according to CHIC perspective 10" ;
    rdfs:subPropertyOf <http://www.chic.eu/ontologies/resource#objectCharacterisedBy> ; 
  rdfs:domain <http://www.chic.eu/ontologies/resource#Model> ;
  rdfs:range rdfs:Resource .
  
<http://www.chic.eu/ontologies/resource#hasPositionIn-11>
  a rdf:Property ;
  rdfs:label "characterised by according to CHIC perspective 11" ;
  rdfs:comment "Associates a model to a concept according to CHIC perspective 11" ;
    rdfs:subPropertyOf <http://www.chic.eu/ontologies/resource#objectCharacterisedBy> ; 
  rdfs:domain <http://www.chic.eu/ontologies/resource#Model> ;
  rdfs:range rdfs:Resource .

<http://www.chic.eu/ontologies/resource#hasPositionIn-12>
  a rdf:Property ;
  rdfs:label "characterised by according to CHIC perspective 12" ;
  rdfs:comment "Associates a model to a concept according to CHIC perspective 12" ;
    rdfs:subPropertyOf <http://www.chic.eu/ontologies/resource#objectCharacterisedBy> ; 
  rdfs:domain <http://www.chic.eu/ontologies/resource#Model> ;
  rdfs:range rdfs:Resource .

<http://www.chic.eu/ontologies/resource#hasPositionIn-13>
  a rdf:Property ;
  rdfs:label "characterised by according to CHIC perspective 13" ;
  rdfs:comment "Associates a model to a concept according to CHIC perspective 13" ;
    rdfs:subPropertyOf <http://www.chic.eu/ontologies/resource#objectCharacterisedBy> ; 
  rdfs:domain <http://www.chic.eu/ontologies/resource#Model> ;
  rdfs:range rdfs:Resource .


# <http://www.chic.eu/ontologies/resource#inputParameterOfModel>    
# <http://www.chic.eu/ontologies/resource#hasFileByFilename>        
# <http://www.chic.eu/ontologies/resource#parameterhasUnits-string> 
# <http://www.chic.eu/ontologies/resource#interpreted-type>         
# <http://www.chic.eu/ontologies/resource#outputParameterOfModel>   
# <http://www.chic.eu/ontologies/resource#hasName>                  
# <http://www.chic.eu/ontologies/resource#modelHasParameter>        
# <http://www.chic.eu/ontologies/resource#modelHasParameter-Input>  
# <http://www.chic.eu/ontologies/resource#modelHasParameter-Output> 
# <http://www.chic.eu/ontologies/resource#parameterOfModel>         
# <http://www.chic.eu/ontologies/resource#parameterhasUnits>        
# <http://www.chic.eu/ontologies/resource#parameterhasDatatype>     
# <http://www.chic.eu/ontologies/resource#objectCharacterisedBy>    
# <http://www.chic.eu/ontologies/resource#hasPositionIn-1>          
# <http://www.chic.eu/ontologies/resource#hasPositionIn-2>          
# <http://www.chic.eu/ontologies/resource#hasPositionIn-3>          
# <http://www.chic.eu/ontologies/resource#hasPositionIn-4>          
# <http://www.chic.eu/ontologies/resource#hasPositionIn-5>          
# <http://www.chic.eu/ontologies/resource#hasPositionIn-6>          
# <http://www.chic.eu/ontologies/resource#hasPositionIn-7>          
# <http://www.chic.eu/ontologies/resource#hasPositionIn-8>          
# <http://www.chic.eu/ontologies/resource#hasPositionIn-9>          
# <http://www.chic.eu/ontologies/resource#hasPositionIn-10>         
# <http://www.chic.eu/ontologies/resource#hasPositionIn-11>         
# <http://www.chic.eu/ontologies/resource#hasPositionIn-12>         
# <http://www.chic.eu/ontologies/resource#hasPositionIn-13> 

### modelling choices oppen
#
#<#model1> rdfs:label "Wilms model" .
#
#<#parameter1>
#  mo:input-parameter-of <#model1> ;
#  rdfs:label "Cell cycle duration of stem cells" ;
#  mo:interpreted-type #<http://www.chic.eu/ontologies/some-domain-ontology#CHIC_0001023> .
#
#<#model2> rdfs:label "not the Wilms model" .
#
#<#parameter2a>
#  mo:input-parameter-of <#model2> ;
#  rdfs:label "Cell cycle duration of stem cells" ;
#  mo:interpreted-type #<http://www.chic.eu/ontologies/some-domain-ontology#CHIC_0001023> .
#
#
#<#model3> rdfs:label "not the Wilms model either" .
#
#<#parameter3a>
#  mo:output-parameter-of <#model3> ;
#  rdfs:label "Cell cycle duration of stem cells" ;
#  mo:interpreted-type #<http://www.chic.eu/ontologies/some-domain-ontology#CHIC_0001023> .
#
#### Independently
# <http://www.chic.eu/ontologies/some-domain-ontology#CHIC_0001023> is defined in a knowledge base as a specialisation of duration (some other ID) of processes of type cell cycle of stem cells (some other id, for a term itself defined as a specialisation of cell cycle involving stem cells)
